LexiToSalt.v
@@ -22,7 +22,13 @@ Fixpoint zip {A: Type} (lst1 lst2 : list A) :=
   | nil, _ => lst2
   | _, nil => lst1
   end.
-
+Definition r0 := nat_reg 0.
+Definition r1 := nat_reg 1.
+Definition r2 := nat_reg 2.
+Definition r3 := nat_reg 3.
+Definition r4 := nat_reg 4.
+Definition r5 := nat_reg 5.
+Definition r6 := nat_reg 6.
 (* -------------- Actual Translations ----------------- *)
 Definition annotation_trans (a:L.annotation) r : instr :=
   match a with
@@ -53,57 +59,55 @@ Definition val_direct_trans (v:L.value)
   end.
 Definition val_trans r (v:value) : instr :=
   match v with
-  | L.var_val (dbjind_var n) => load r sp false n
+  | L.var_val (dbjind_var n) => load r sp n
   | _ => mov r (val_direct_trans v [])
   end.
 
 Definition expr_trans exp : list instr :=
   match exp with
-  | L.val_e v =>  [val_trans 1 v]
+  | L.val_e v =>  [val_trans r1 v]
   | L.add v1 v2 =>
-    [val_trans 1 v1; val_trans 2 v2; add 1 (reg_o 2)]
+    [val_trans r1 v1; val_trans r2 v2; add r1 r2]
   | L.app v lst => 
-    ([val_trans 0 v] ++
+    ([val_trans r0 v] ++
     (rev (zip_map (val_trans)
       (map nat_reg (iota (List.length lst)))
       lst))
-    ++ [call (reg_o 0)])
+    ++ [call r0])
   | L.newref h_v =>
-    ([malloc 1 (List.length h_v)] ++
-    zip (map (val_trans 2) h_v)
-      (map (fun x => store 1 (x-1) (reg_o 2))
+    ([malloc r1 (List.length h_v)] ++
+    zip (map (val_trans r2) h_v)
+      (map (fun x => store r1 (x-1) r2)
         (iota (List.length h_v))))
-  | L.pi i v => [val_trans 1 v; load 1 1 true i]
+  | L.pi i v => [val_trans r1 v; load r1 r1 i]
   | L.asgn v1 i v2 =>
-    [val_trans 1 v2; val_trans 2 v1; store 2 i (reg_o 1)]
+    [val_trans r1 v2; val_trans r2 v1; store r2 i r1]
   | L.handle (L.c_lab clab_body)
     (L.c_lab clab_op) A v_env =>
-    [annotation_trans A 4; val_trans 3 v_env;
-      mov 2 (cloc clab_op 0); mov 1 (cloc clab_body 0);
-      call (match A with 
-      | L.general => (cloc "handle"%string 0)
-      | _ => (cloc "handle_same_stack"%string 0) end)]
-  | L.raise L.general v1 v2 => [val_trans 2 v2; val_trans 1 v1;
+    [annotation_trans A r4; val_trans r3 v_env;
+      mov r2 (cloc clab_op 0); mov r1 (cloc clab_body 0);
+     call (if a_eqb L.general A
+           then cloc "handle"%string 0
+           else cloc "handle_same_stack"%string 0)]
+  | L.raise L.general v1 v2 => [val_trans r2 v2; val_trans r1 v1;
     call (cloc "raise"%string 0)]
-  | L.raise L.tail v1 v2 => [val_trans 2 v2 ; val_trans 1 v1;
-    load 3 1 false 3; load 1 1 false 2 ; call (reg_o 3)]
-  | L.resume v1 v2 => [val_trans 2 v2 ; val_trans 1 v1;
+  | L.raise L.tail v1 v2 => [val_trans r2 v2 ; val_trans r1 v1;
+    load r3 r1 3; load r1 r1 2 ; call r3]
+  | L.resume v1 v2 => [val_trans r2 v2 ; val_trans r1 v1;
     call (cloc "resume"%string 0)]
   (* Impossible case for newref continuation *)
   | _ => []
   end.
 Fixpoint term_trans tm : list instr:=
   match tm with
-  | L.val_term v => [val_trans 1 v]
+  | L.val_term v => [val_trans r1 v]
   | L.bind (L.raise L.abort v1 v2) t =>
-    [val_trans 2 v2 ; val_trans 1 v1;
-    load 3 1 false 3; mov sp (reg_o 1); load 1 1 false 2;
-    sfree 4; jmp (reg_o 3)]
-  | L.bind (L.exit v) t =>
-    [val_trans 1 v; halt]
+    [val_trans r2 v2 ; val_trans r1 v1;
+    load r3 r1 3; mov sp r1; load r1 r1 2;
+    sfree 4; jmp r3]        
   | L.bind exp t =>
     expr_trans exp
-    ++ [push (reg_o 1)]
+    ++ [push r1]
     ++ term_trans t
   (* special case, not needed for translating code,
      but needed for relating lexi and salt's config *)
@@ -124,15 +128,17 @@ Definition func_term_trans (n:nat) (t:L.term) : list instr :=
   | _ => [sfree (n + (num_let t)); ret]
   end.
 Definition func_trans (f:L.function) : instr_seq :=
-  match f with L.func n t =>
-    ins_seq
-    (map (fun (x:nat) => (push (reg_o x)))
-      (List.rev (iota n))
-    ++ func_term_trans n t)
+  match f with
+  | L.func n t =>
+      ins_seq
+        ((map (fun x => push (nat_reg x))
+           (iota n))
+           ++ func_term_trans n t)
+  | L.ns_func => S.ns_ins_seq
   end.
-Definition code_trans (c:L.code) : S.program :=
+Definition code_mem_trans (c:L.code_mem) : S.code_mem :=
   fun (x:code_loc) =>
-  match x with cloc_str str => func_trans (c str) end.
+  match x with cloc_str str => func_trans (c str) end.  
 
 (*
 All changes made
