SimProof.v
@@ -16,12 +16,12 @@ Delimit Scope Lexi_scope with L_scope.
                           Simulation 
    ---------------------------------------------------------- *)
 Definition multi : forall A : Type, Relation_Definitions.relation A ->
-  A -> A -> Prop := Relation_Operators.clos_refl_trans_1n.
+                                    A -> A -> Prop := Relation_Operators.clos_refl_trans_1n.
 Arguments multi {A}.
 Inductive multi_plus {X : Type} (R : X -> X -> Prop) : X -> X -> Prop :=
-  | multi_one_step : forall (x y : X), R x y -> multi_plus R x y
-  | multi_step : forall (x y z : X),
-      R x y -> multi_plus R y z -> multi_plus R x z.
+| multi_one_step : forall (x y : X), R x y -> multi_plus R x y
+| multi_step : forall (x y z : X),
+    R x y -> multi_plus R y z -> multi_plus R x z.
 (* -----------------------------------------------------------------
     Theorem 2: translation from lexi to salt is semantic preserving
    ----------------------------------------------------------------- *)
@@ -29,18 +29,16 @@ Inductive multi_plus {X : Type} (R : X -> X -> Prop) : X -> X -> Prop :=
   the 3 conditions *)
 
 
-Theorem cond1 : forall C1 C2 M1 M2 main_lab init_lab,
-  code_trans C1 = C2 ->
-  init_L (c_lab init_lab) (letrec C1 (bind (app (c_lab main_lab) [])
-    (bind (exit (var_val 0)) (val_term 0)))) M1
-  -> init_S (cloc_str init_lab) (cloc_str main_lab) C2 M2 -> LS_rel M1 M2.
+Theorem cond1 : forall C1 C2 M1 M2,
+    code_mem_trans C1 = C2 -> init_L C1 M1 ->
+    init_S C2 M2 -> LS_rel M1 M2.
 Proof with super_a.
   intros. destruct M1 as [[[[LC LH] LK] LE] Lt], M2 as [[SC SH] SR].
   inversion H1... inversion H0...
   apply rel_LS with
-    (SIlst:=[mov 0 (cloc main_lab 0); call (reg_o 0);
-             push (reg_o 1); load 1 sp false 0; halt])
+    (SIlst:=func_term_trans 0 L_init_tm)
     (lst:=[])...
+  - intros. destruct H...
   - destruct L_stack as [L_stack_str].
     apply rel_env_context with
       (s_out:=[ns_hloc;int_w 0; ns_hloc; ns_cloc])...
@@ -54,22 +52,26 @@ Proof with super_a.
       (L_prev:=""%string) (s_prev:=[]).
   - intros... cbv in H. injection H. intros...
   - extensionality x. destruct x as [str]. 
-    unfold c_update,L.c_update.
-    unfold c_eqb,L.c_eqb.
-    destruct (eqb init_lab str) as []eqn:?;cbn;rewrite Heqb...
-  - intros. unfold wf_func_tm,L.c_update.
-    destruct (L.c_eqb init_lab x)...
-    specialize H12 with x. unfold wf_func_tm in H12...
-  - unfold c_update... rewrite eqb_refl...
-    (*- repeat apply_fresh lc_bind...*)
+    unfold c_comp,L.c_comp,code_mem_trans...
+    destruct (L_init_func str)... 
+  - intros. unfold L.c_comp.
+    destruct (L_init_func x) as []eqn:?...
+    unfold L_init_func in Heqf.
+    unfold L.c_update in Heqf.
+    destruct (L.c_eqb exit_lab x).
+    + inversion Heqf...
+    + destruct (L.c_eqb init_lab x).
+      * inversion Heqf... intros. destruct H...
+      * inversion Heqf...
+        (*- repeat apply_fresh lc_bind...*)
 Qed.
 
 Theorem cond2 : forall M1 M2 i,
-  LS_rel M1 M2 -> final_L M1 i -> final_S M2 i.
+    LS_rel M1 M2 -> final_L M1 i -> final_S M2 i.
 Proof with automate.
   intros. destruct M1 as [[[[LC LH] LK] LE] Lt], M2 as [[SC SH] SR].
   inversion H0... inversion H... inversion H10...
-  simpl. rewrite H13. inversion H9... apply nth_middle.
+  cbn. rewrite H13. inversion H8... apply nth_middle.
 Qed.
 
 Definition un_tuple (tup:tuple_heap_val) : list word :=
@@ -86,16 +88,16 @@ Lemma stack_un_stack : forall lst,
     stack (un_stack (stack lst)) = stack lst.
 Proof with automate. intros... Qed.
 Lemma term_trans_not_nil : forall tm,
-  term_trans tm <> [].
+    term_trans tm <> [].
 Proof with automate.
   intros. unfold not. destruct tm;simpl...
   destruct e;intros;simpl;apply eq_sym in H;
-  generalize dependent H...
+    generalize dependent H...
   - apply app_cons_not_nil.
   - destruct a...
 Qed.
 Lemma ins_verify : forall (A : Type) (l l' : list A) (d : A) (n : nat),
-       nth (n + Datatypes.length l) (l ++ l') d = nth n l' d.
+    nth (n + List.length l) (l ++ l') d = nth n l' d.
 Proof.
   intros. rewrite PeanoNat.Nat.add_comm.
   apply app_nth2_plus.
@@ -110,7 +112,16 @@ Proof with super_a.
   rewrite app_nth1... specialize H with n.
   rewrite map_length...  
 Qed.
-(*Lemma update_nth_map: forall {A B:Type} ind (f:A->B) lst v,
+
+(*Lemma push1_before_tm : forall ft lst Ilst E t,
+          wf_func_tm ft ->
+          func_trans ft = ins_seq (lst ++ Ilst) ->
+          LS_rel_ins (E,t) (ins_seq (tl Ilst)) ->
+          nth 0 Ilst ns_ins = push (reg_o 1).
+Proof with super_a.
+  intros. 
+
+  Lemma update_nth_map: forall {A B:Type} ind (f:A->B) lst v,
     update_nth ind (List.map f lst) (f v)
     = (List.map f (L.update_nth ind lst v)).
 Proof with super_a.
@@ -118,169 +129,168 @@ intros. Search (List.map _ _=_(List.map _ _)). Admitted.
   Lemma Sn_n1 : forall n m, S n = n + 1.
 Proof. intros.  Qed.
 Lemma SSn_n2 : forall n, S (S n) = n + 2.*)
-  
+
 Theorem cond3 : forall LC SC H1 K1 E1 t1 R2 H2 H1' K1' E1' t1',
-  LS_rel (LC, H1, K1, E1, t1)
-    (SC, H2, R2) ->
-  L.step LC (H1, K1, E1, t1) (H1', K1', E1', t1') ->
-  (exists H2' R2',
-    multi_plus (S.step SC)
-      (H2, R2) (H2', R2') /\
-    LS_rel (LC, H1', K1', E1', t1') (SC, H2', R2')).
+    LS_rel (LC, H1, K1, E1, t1)
+      (SC, H2, R2) ->
+    L.step LC (H1, K1, E1, t1) (H1', K1', E1', t1') ->
+    (exists H2' R2',
+        multi_plus (S.step SC)
+          (H2, R2) (H2', R2') /\
+          LS_rel (LC, H1', K1', E1', t1') (SC, H2', R2')).
 Proof with super_a.
   intros. inversion H... inversion H12...
   inversion H0;automate;
     remember (List.map run_cst_trans E1 ++ s_out) as cur_stk_val;
     remember (cloc Clab (List.length lst)) as l;
     remember ((L_out,stack cur_stk_val)::H_stack) as cur_stkh;
-    remember [(nat_reg 3,o3);(nat_reg 4,o4);(nat_reg 5,o5);
-              (nat_reg 6,o6)] as R36.
+    remember [(r3,o3);(r4,o4);(r5,o5);
+              (r6,o6)] as R36.
   (* 14 stepping rules, prove the multi and rel for each *)
-   - (* x = v1 + v2 *) exists
+  - (* x = v1 + v2 *) exists
       ((L_out,stack ((int_w (i1+i2)) :: cur_stk_val))
-        :: H_stack,SH_tup,SH_conts),
+         :: H_stack,SH_tup,SH_conts),
       ([(ip,loc_w (incr_cloc 4 l));(sp,loc_w (hloc L_out
-        (1+(List.length cur_stk_val))));
-        (nat_reg 0,o0);
-        (nat_reg 1,int_w (i1+i2));(nat_reg 2,int_w i2)]
-      ++ R36). split.
+                                                (1+(List.length cur_stk_val))));
+        (r0,o0);
+        (r1,int_w (i1+i2));(r2,int_w i2)]
+         ++ R36). split.
     (* stepping translated salt code for addition *)
     + apply multi_step with (*y is 1 step after current*)
-      (y:=((cur_stkh,SH_tup,SH_conts),
-            [(ip,loc_w (next_cloc l));
-             (sp,loc_w (hloc L_out (List.length cur_stk_val)));
-             (nat_reg 0,o0);(nat_reg 1,int_w i1);
-             (nat_reg 2,o2)] ++ R36)).
+        (y:=((cur_stkh,SH_tup,SH_conts),
+              [(ip,loc_w (next_cloc l));
+               (sp,loc_w (hloc L_out (List.length cur_stk_val)));
+               (r0,o0);(r1,int_w i1);
+               (r2,o2)] ++ R36)).
       { apply S_mov with
-          (d:=1) (o:=i1)
+          (d:=r1) (o:=i1)
           (R:=[(ip,loc_w l);
                (sp,loc_w (hloc L_out (List.length cur_stk_val)));
-               (nat_reg 0,o0);(nat_reg 1,o1);
-               (nat_reg 2,o2)] ++ R36)...
-        inversion H11. rewrite H15... apply nth_middle. }
+               (r0,o0);(r1,o1);
+               (r2,o2)] ++ R36)...
+        rewrite H15. inversion H10... apply nth_middle. }
       apply multi_step with
         (y:=((cur_stkh,SH_tup,SH_conts),
               [(ip,loc_w (incr_cloc 2 l));
                (sp,loc_w (hloc L_out (List.length cur_stk_val)));
-               (nat_reg 0,o0);(nat_reg 1,int_w i1);
-               (nat_reg 2,int_w i2)] ++ R36)).
+               (r0,o0);(r1,int_w i1);
+               (r2,int_w i2)] ++ R36)).
       { apply S_mov with
-          (d:=2) (o:=i2)
+          (d:=r2) (o:=i2)
           (R:=[(ip,loc_w (next_cloc l));
                (sp,loc_w (hloc L_out (List.length cur_stk_val)));
-               (nat_reg 0,o0);(nat_reg 1,int_w i1);
-               (nat_reg 2,o2)] ++ R36)...
-        inversion H11. rewrite H15...
+               (r0,o0);(r1,int_w i1);
+               (r2,o2)] ++ R36)...
+        inversion H10. rewrite H15...
         apply ins_verify with (n:=1). }
       apply multi_step with
         (y:=((cur_stkh,SH_tup,SH_conts),
               [(ip,loc_w (incr_cloc 3 l));
                (sp,loc_w (hloc L_out (List.length cur_stk_val)));
-               (nat_reg 0,o0);(nat_reg 1,int_w (i1+i2));
-               (nat_reg 2,int_w i2)] ++ R36)).
+               (r0,o0);(r1,int_w (i1+i2));
+               (r2,int_w i2)] ++ R36)).
       { apply S_add with
-          (reg:=nat_reg 1)
-          (o:=reg_o (nat_reg 2))
+          (reg:=r1)
+          (o:=r2)
           (R:=[(ip,loc_w (incr_cloc 2 l));
                (sp,loc_w (hloc L_out (List.length cur_stk_val)));
-               (nat_reg 0,o0);(nat_reg 1,int_w i1);
-               (nat_reg 2,int_w i2)] ++ R36)... rewrite H15. inversion H11...
+               (r0,o0);(r1,int_w i1);
+               (r2,int_w i2)] ++ R36)... rewrite H15. inversion H10...
         apply ins_verify with (n:=2). }
       constructor.
       apply S_push with
-        (o:=reg_o (nat_reg 1))
+        (o:=r1)
         (R:=[(ip,loc_w (incr_cloc 3 l));
              (sp,loc_w (hloc L_out (List.length cur_stk_val)));
-             (nat_reg 0,o0);(nat_reg 1,int_w (i1+i2));
-             (nat_reg 2,int_w i2)] ++ R36)...
-      rewrite H15. inversion H11... apply ins_verify with (n:=3).
+             (r0,o0);(r1,int_w (i1+i2));
+             (r2,int_w i2)] ++ R36)...
+      rewrite H15. inversion H10... apply ins_verify with (n:=3).
     (* prove LS_rel for L_add *)
     + unfold incr_cloc,next_cloc... apply rel_LS with
-      (lst:=lst ++ firstn 4 SIlst)
-      (SIlst:= tl (tl (tl (tl SIlst))));inversion H11...
+        (lst:=lst ++ firstn 4 SIlst)
+        (SIlst:= tl (tl (tl (tl SIlst))));inversion H10...
       * pose proof term_trans_not_nil as NN. specialize NN with
           (tm:=t1'). cbn. destruct (RelConfig.LS.term_trans t1')as []eqn:?;automate.
-        rewrite <- Heql. rewrite <- PeanoNat.Nat.add_succ_comm...        
+        rewrite <- Heql. rewrite <- PeanoNat.Nat.add_succ_comm...
+        inversion H2...
       * apply rel_env_context with (s_out:=s_out)...
       * rewrite H15... assert (AssocIns: forall (x1:instr) x2 x3 x4 tl,
-          [x1;x2;x3;x4] ++ tl = x1::x2::x3::x4::tl). { intros... }
+                                  [x1;x2;x3;x4] ++ tl = x1::x2::x3::x4::tl). { intros... }
         rewrite <- AssocIns,app_assoc...
       * rewrite app_length. rewrite PeanoNat.Nat.add_comm...
-      * destruct t1';inversion H17...
   - (* x = v *) exists
       ((L_out,stack ((val_direct_trans v cur_stk_val) :: cur_stk_val))
-        :: H_stack,SH_tup,SH_conts),
+         :: H_stack,SH_tup,SH_conts),
       ([(ip,loc_w (incr_cloc 2 l));
         (sp,loc_w (hloc L_out (1+(List.length cur_stk_val))));
-        (nat_reg 0,o0);
-        (nat_reg 1,val_direct_trans v cur_stk_val);
-        (nat_reg 2,o2)] ++ R36). split.
+        (r0,o0);
+        (r1,val_direct_trans v cur_stk_val);
+        (r2,o2)] ++ R36). split.
     + (* stepping translated salt code for single value *)
       apply multi_step with (*y is 1 step after current*)
-      (y:=((cur_stkh,SH_tup,SH_conts),
-            [(ip,loc_w (next_cloc l));
-             (sp,loc_w (hloc L_out (List.length cur_stk_val)));
-             (nat_reg 0,o0);
-             (nat_reg 1,val_direct_trans v cur_stk_val);
-             (nat_reg 2,o2)] ++ R36)).
-      { destruct v as [cst|[ind|str]].
-        - apply S_mov with (d:=1)
-        (o:=val_direct_trans (const_val cst) cur_stk_val)
-        (R:=[(ip,loc_w l);
-             (sp,loc_w (hloc L_out (List.length cur_stk_val)));
-             (nat_reg 0,o0);(nat_reg 1,o1);
-             (nat_reg 2,o2)] ++ R36)...
-        inversion H11... rewrite H15... apply nth_middle.
-        - pose proof S_load_stk as Ins. specialize Ins with
-          (d:=1) (s:=sp) (off:=ind)
-          (L:=L_out) (sign:=false)
-          (lst:=cur_stk_val) (i:=List.length cur_stk_val)
-          (R:=[(ip,loc_w l);
+        (y:=((cur_stkh,SH_tup,SH_conts),
+              [(ip,loc_w (next_cloc l));
                (sp,loc_w (hloc L_out (List.length cur_stk_val)));
-               (nat_reg 0,o0);(nat_reg 1,o1);
-               (nat_reg 2,o2)] ++ R36).
-          rewrite PeanoNat.Nat.sub_diag in Ins.
-          destruct SH_conts. apply Ins...
-          + inversion H11. rewrite H15... apply nth_middle.
-          + rewrite h_eqb_refl...
-        - apply S_mov with
-            (d:=1) (o:=val_direct_trans (var_val str) cur_stk_val)
+               (r0,o0);
+               (r1,val_direct_trans v cur_stk_val);
+               (r2,o2)] ++ R36)).
+      { destruct v as [cst|[ind|str]].
+        - apply S_mov with (d:=r1)
+                           (o:=val_direct_trans (const_val cst) cur_stk_val)
+                           (R:=[(ip,loc_w l);
+                                (sp,loc_w (hloc L_out (List.length cur_stk_val)));
+                                (r0,o0);(r1,o1);
+                                (r2,o2)] ++ R36)...
+          inversion H10... rewrite H15... apply nth_middle.
+        - pose proof S_load_sp as Ins. specialize Ins with
+            (d:=r1) (off:=ind)
+            (L:=L_out)
+            (lst:=cur_stk_val) (i:=List.length cur_stk_val)
             (R:=[(ip,loc_w l);
                  (sp,loc_w (hloc L_out (List.length cur_stk_val)));
-                 (nat_reg 0,o0);(nat_reg 1,o1);
-                 (nat_reg 2,o2)] ++ R36)...
-        inversion H11... rewrite H15... apply nth_middle. }
+                 (r0,o0);(r1,o1);
+                 (r2,o2)] ++ R36).
+          rewrite PeanoNat.Nat.sub_diag in Ins.
+          apply Ins...
+          + inversion H10. rewrite H15... apply nth_middle.
+          + rewrite h_eqb_refl...
+        - apply S_mov with
+            (d:=r1) (o:=val_direct_trans (var_val str) cur_stk_val)
+            (R:=[(ip,loc_w l);
+                 (sp,loc_w (hloc L_out (List.length cur_stk_val)));
+                 (r0,o0);(r1,o1);
+                 (r2,o2)] ++ R36)...
+          inversion H10... rewrite H15... apply nth_middle. }
       constructor.
       apply S_push with
-        (o:=reg_o 1)
+        (o:=r1)
         (R:=[(ip,loc_w (next_cloc l));
-             (sp,loc_w(hloc L_out (Datatypes.length cur_stk_val)));
-             (nat_reg 0,o0);
-             (nat_reg 1,val_direct_trans v cur_stk_val);
-             (nat_reg 2,o2)] ++ R36)...
-      rewrite H15. inversion H11...
+             (sp,loc_w(hloc L_out (List.length cur_stk_val)));
+             (r0,o0);
+             (r1,val_direct_trans v cur_stk_val);
+             (r2,o2)] ++ R36)...
+      rewrite H15. inversion H10...
       apply ins_verify with (n:=1).
     + (* prove LS_rel for x=v *)
       rewrite Heql. rewrite HeqR36. apply rel_LS with
         (lst:=lst ++ firstn 2 SIlst) (SIlst:= tl (tl SIlst))...
-      * inversion H11... pose proof term_trans_not_nil as NN.
+      * inversion H10... pose proof term_trans_not_nil as NN.
         specialize NN with (tm:=t1'). destruct
-        (RelConfig.LS.term_trans t1')as []eqn:?;automate. rewrite <- Heql.
+          (RelConfig.LS.term_trans t1')as []eqn:?;automate. rewrite <- Heql.
         rewrite <- PeanoNat.Nat.add_succ_comm.
-        apply rel_tm with (E:=L.var_deref E1 v :: E1) (t:=t1').
+        apply rel_ins. inversion H2...
       * apply rel_env_context with (s_out:=s_out)...
         destruct v as [cst|[ind|str]]...
         rewrite <- map_nth with (d:=L.ns). rewrite app_nth1...
-        inversion H17... inversion H4... inversion H2...
-        rewrite List.map_length...
+        rewrite map_length.
+        inversion H10... inversion H2...
+        inversion H6... inversion H3...
       * rewrite H15. destruct SIlst... destruct SIlst...
         rewrite <- app_assoc. assert (AssocIns: forall (x1:instr) x2 tl,
-          [x1;x2] ++ tl = x1::x2::tl). { intros... }
+                                         [x1;x2] ++ tl = x1::x2::tl). { intros... }
         rewrite <- AssocIns...
       * destruct SIlst... destruct SIlst...
-        rewrite app_length. rewrite PeanoNat.Nat.add_comm...
-      * destruct t1';inversion H17...
-        
+        rewrite app_length. rewrite PeanoNat.Nat.add_comm... 
   - (* x = newref<v> *)
     destruct L as [L_str].
     exists ((L_out,
@@ -289,124 +299,123 @@ Proof with super_a.
                tuple ([val_direct_trans v cur_stk_val]); SH_tup,SH_conts),
       ([(ip,loc_w (incr_cloc 4 l));
         (sp,loc_w (hloc L_out (1+(List.length cur_stk_val))));
-        (nat_reg 0,o0);
-        (nat_reg 1,loc_w (hloc L_str 0));
-        (nat_reg 2,val_direct_trans v cur_stk_val)]
-      ++ R36). split.
-      (* stepping salt code for newref *)
+        (r0,o0);
+        (r1,loc_w (hloc L_str 0));
+        (r2,val_direct_trans v cur_stk_val)]
+         ++ R36). split.
+    (* stepping salt code for newref *)
     + apply multi_step with
         (y:=((cur_stkh,
-                hloc_str L_str !->t
-                  tuple ([ns]);SH_tup,SH_conts),
+               hloc_str L_str !->t
+                 tuple ([ns]);SH_tup,SH_conts),
               [(ip,loc_w (next_cloc l));
                (sp,loc_w (hloc L_out (List.length cur_stk_val)));
-               (nat_reg 0,o0);
-               (nat_reg 1,loc_w (hloc L_str 0));
-               (nat_reg 2,o2)] ++ R36)).
+               (r0,o0);
+               (r1,loc_w (hloc L_str 0));
+               (r2,o2)] ++ R36)).
       { apply S_malloc with
-          (i:=1) (d:=1)
+          (i:=1) (d:=r1)
           (R:=[(ip,loc_w l);
                (sp,loc_w (hloc L_out (List.length cur_stk_val)));
-                (nat_reg 0,o0);
-               (nat_reg 1,o1);(nat_reg 2,o2)] ++ R36)...
-        - rewrite H15. inversion H11... apply nth_middle. }
+               (r0,o0);
+               (r1,o1);(r2,o2)] ++ R36)...
+        - rewrite H15. inversion H10... apply nth_middle. }
       apply multi_step with
         (y:=((cur_stkh,
-                hloc_str L_str !->t
-                  tuple ([ns]);SH_tup,SH_conts),
+               hloc_str L_str !->t
+                 tuple ([ns]);SH_tup,SH_conts),
               [(ip,loc_w (incr_cloc 2 l));
                (sp,loc_w (hloc L_out (List.length cur_stk_val)));
-               (nat_reg 0,o0);
-               (nat_reg 1,loc_w (hloc L_str 0));
-               (nat_reg 2,val_direct_trans v cur_stk_val)]
-        ++ R36)).
+               (r0,o0);
+               (r1,loc_w (hloc L_str 0));
+               (r2,val_direct_trans v cur_stk_val)]
+                ++ R36)).
       { destruct v as [cst|[ind|str]].
         - apply S_mov with
-            (d:=2) (o:=val_direct_trans (const_val cst) cur_stk_val)
+            (d:=r2) (o:=val_direct_trans (const_val cst) cur_stk_val)
             (R:=[(ip,loc_w (next_cloc l));
                  (sp,loc_w (hloc L_out (List.length cur_stk_val)));
-                 (nat_reg 0,o0);
-                 (nat_reg 1,loc_w (hloc L_str 0));
-                 (nat_reg 2,o2)] ++ R36)...
-          rewrite H15. inversion H11...
+                 (r0,o0);
+                 (r1,loc_w (hloc L_str 0));
+                 (r2,o2)] ++ R36)...
+          rewrite H15. inversion H10...
           apply ins_verify with (n:=1).
-        - pose proof S_load_stk as Ins. specialize Ins with
-            (d:=2) (s:=sp) (off:=ind)
-            (L:=L_out) (sign:=false)
+        - pose proof S_load_sp as Ins. specialize Ins with
+            (d:=r2) (off:=ind)
+            (L:=L_out)
             (lst:=cur_stk_val) (i:=List.length cur_stk_val)
             (R:=[(ip,loc_w (next_cloc l));
                  (sp,loc_w (hloc L_out (List.length cur_stk_val)));
-                 (nat_reg 0,o0);
-                 (nat_reg 1,loc_w (hloc L_str 0));
-                 (nat_reg 2,o2)] ++ R36).
+                 (r0,o0);
+                 (r1,loc_w (hloc L_str 0));
+                 (r2,o2)] ++ R36).
           rewrite PeanoNat.Nat.sub_diag in Ins.
-          destruct SH_conts. apply Ins...
-          + inversion H11. rewrite H15... apply ins_verify with (n:=1).
+          apply Ins...
+          + inversion H10. rewrite H15... apply ins_verify with (n:=1).
           + rewrite h_eqb_refl...
         - apply S_mov with
-            (d:=2) (o:=val_direct_trans (var_val str) cur_stk_val)
+            (d:=r2) (o:=val_direct_trans (var_val str) cur_stk_val)
             (R:=[(ip,loc_w (next_cloc l));
                  (sp,loc_w (hloc L_out (List.length cur_stk_val)));
-                 (nat_reg 0,o0);
-                 (nat_reg 1,loc_w (hloc L_str 0));
-                 (nat_reg 2,o2)] ++ R36)...
-      rewrite H15. inversion H11... apply ins_verify with (n:=1). }
+                 (r0,o0);
+                 (r1,loc_w (hloc L_str 0));
+                 (r2,o2)] ++ R36)...
+          rewrite H15. inversion H10... apply ins_verify with (n:=1). }
       apply multi_step with
         (y:=((cur_stkh,
-                hloc_str L_str !->t
-                  tuple ([val_direct_trans v cur_stk_val]);SH_tup,SH_conts),
+               hloc_str L_str !->t
+                 tuple ([val_direct_trans v cur_stk_val]);SH_tup,SH_conts),
               [(ip,loc_w (incr_cloc 3 l));
                (sp,loc_w (hloc L_out (List.length cur_stk_val)));
-               (nat_reg 0,o0);
-               (nat_reg 1,loc_w (hloc L_str 0));
-               (nat_reg 2,val_direct_trans v cur_stk_val)]
-        ++ R36)).
+               (r0,o0);
+               (r1,loc_w (hloc L_str 0));
+               (r2,val_direct_trans v cur_stk_val)]
+                ++ R36)).
       { pose proof S_store as Ins. specialize Ins with
-          (d:=1) (o:=reg_o 2) (j:=0) (L:=hloc_str L_str)
+          (d:=r1) (o:=reg_o r2) (j:=0) (L:=hloc_str L_str)
           (H_tup:= L_str !->t tuple [ns]; SH_tup) (lst:=[ns])
           (R:=[(ip,loc_w (incr_cloc 2 l));
                (sp,loc_w (hloc L_out (List.length cur_stk_val)));
-               (nat_reg 0,o0);
-               (nat_reg 1,loc_w (hloc L_str 0));
-               (nat_reg 2,val_direct_trans v cur_stk_val)] ++ R36).
+               (r0,o0);
+               (r1,loc_w (hloc L_str 0));
+               (r2,val_direct_trans v cur_stk_val)] ++ R36).
         rewrite heap_front_update in Ins. apply Ins...
-        - rewrite H15. inversion H11.
+        - rewrite H15. inversion H10.
           apply ins_verify with (n:=2).
         - unfold th_update. rewrite h_eqb_refl... }
       constructor.
       apply S_push with
-        (o:=reg_o (nat_reg 1))
+        (o:=r1)
         (R:=[(ip,loc_w (incr_cloc 3 l));
              (sp,loc_w (hloc L_out (List.length cur_stk_val)));
-             (nat_reg 0,o0);
-             (nat_reg 1,loc_w (hloc L_str 0));
-             (nat_reg 2,val_direct_trans v cur_stk_val)] ++ R36)...
-      rewrite H15. inversion H11... apply ins_verify with (n:=3).
+             (r0,o0);
+             (r1,loc_w (hloc L_str 0));
+             (r2,val_direct_trans v cur_stk_val)] ++ R36)...
+      rewrite H15. inversion H10... apply ins_verify with (n:=3).
     + (* Prove LS_rel for newref *)
       unfold incr_cloc,next_cloc... apply rel_LS with
-      (lst:=lst ++ firstn 4 SIlst)
-      (SIlst:= tl (tl (tl (tl SIlst))));inversion H11;automate.
+        (lst:=lst ++ firstn 4 SIlst)
+        (SIlst:= tl (tl (tl (tl SIlst))));inversion H10;automate.
       * pose proof term_trans_not_nil as NN. specialize NN with
-        (tm:=t1'). cbn. destruct (RelConfig.LS.term_trans t1')as []eqn:?;automate.
+          (tm:=t1'). cbn. destruct (RelConfig.LS.term_trans t1')as []eqn:?;automate.
         rewrite <- Heql. rewrite <- PeanoNat.Nat.add_succ_comm.
-        apply rel_tm with (E:=L.d_lab_const (L.obj_lab L_str) :: E1) (t:=t1').
+        apply rel_ins. inversion H10... inversion H3...
       * apply rel_env_context with (s_out:=s_out)...
       * unfold th_update,L.th_update,L.h_eqb,h_eqb.
         intros. destruct (String.eqb L_str L_tup)...
         -- inversion H1... destruct v as [|[|]]...
            rewrite <- map_nth with (d:=L.ns)...
-           rewrite app_nth1... inversion H17...
-           inversion H7...
-           specialize H3 with (v:=L.var_val n).
+           rewrite app_nth1... inversion H2...
+           inversion H8...
+           specialize H6 with (v:=L.var_val n).
            assert (Temp:In (L.var_val n) [L.var_val (L.dbjind_var n)]).
-           { super_a. } apply H3 in Temp. inversion Temp...
+           { super_a. } apply H6 in Temp. inversion Temp...
            rewrite List.map_length...
-        -- inversion H13... inversion H3...
+        -- inversion H13... inversion H6...
       * rewrite H15... assert (AssocIns: forall (x1:instr) x2 x3 x4 tl,
-          [x1;x2;x3;x4] ++ tl = x1::x2::x3::x4::tl). { intros... }
+                                  [x1;x2;x3;x4] ++ tl = x1::x2::x3::x4::tl). { intros... }
         rewrite <- AssocIns,app_assoc...
       * rewrite app_length. rewrite PeanoNat.Nat.add_comm...
-      * destruct t1';inversion H17...
   - (* x = pi_i(v)*)
     destruct L as [L_str].
     exists ((L_out,
@@ -414,86 +423,86 @@ Proof with super_a.
               :: H_stack,SH_tup,SH_conts),
       ([(ip,loc_w (incr_cloc 3 l));
         (sp,loc_w (hloc L_out (1+(List.length cur_stk_val))));
-        (nat_reg 0,o0);
-        (nat_reg 1,nth i (List.map run_cst_trans lst0) ns);
-        (nat_reg 2,o2)] ++ R36). split.
+        (r0,o0);
+        (r1,nth i (List.map run_cst_trans lst0) ns);
+        (r2,o2)] ++ R36). split.
     (* stepping salt code for loading from heap *)
     + apply multi_step with
         (y:=((cur_stkh,SH_tup,SH_conts),
               [(ip,loc_w (next_cloc l));
                (sp,loc_w (hloc L_out (List.length cur_stk_val)));
-               (nat_reg 0,o0);
-               (nat_reg 1,val_direct_trans v cur_stk_val);
-               (nat_reg 2,o2)] ++ R36)).
+               (r0,o0);
+               (r1,val_direct_trans v cur_stk_val);
+               (r2,o2)] ++ R36)).
       { destruct v as [cst|[ind|str]].
         - apply S_mov with
-            (d:=1) (o:=val_direct_trans (const_val cst) cur_stk_val) (l:=l)
+            (d:=r1) (o:=val_direct_trans (const_val cst) cur_stk_val) (l:=l)
             (R:=[(ip,loc_w l);(sp,loc_w (hloc L_out (List.length cur_stk_val)));
-                 (nat_reg 0,o0);(nat_reg 1,o1);
-                 (nat_reg 2,o2)] ++ R36)...
-        - pose proof S_load_stk as Ins. specialize Ins with
-            (d:=1) (s:=sp) (off:=ind) (L:=L_out) (sign:=false)
+                 (r0,o0);(r1,o1);
+                 (r2,o2)] ++ R36)...
+        - pose proof S_load_sp as Ins. specialize Ins with
+            (d:=r1) (off:=ind) (L:=L_out) 
             (lst:=cur_stk_val) (i:=List.length cur_stk_val)
             (R:=[(ip,loc_w l);(sp,loc_w (hloc L_out (List.length cur_stk_val)));
-                 (nat_reg 0,o0);(nat_reg 1,o1);
-                 (nat_reg 2,o2)] ++ R36).
-          rewrite PeanoNat.Nat.sub_diag in Ins. destruct SH_conts.
+                 (r0,o0);(r1,o1);
+                 (r2,o2)] ++ R36).
+          rewrite PeanoNat.Nat.sub_diag in Ins. 
           apply Ins...
-          + inversion H11. rewrite H15... apply nth_middle.
+          + inversion H10. rewrite H15... apply nth_middle.
           + rewrite h_eqb_refl...
         - apply S_mov with
-            (d:=1) (o:=val_direct_trans (var_val str) cur_stk_val)
+            (d:=r1) (o:=val_direct_trans (var_val str) cur_stk_val)
             (R:=[(ip,loc_w l);(sp,loc_w (hloc L_out (List.length cur_stk_val)));
-                 (nat_reg 0,o0);(nat_reg 1,o1);
-                 (nat_reg 2,o2)] ++ R36)... }
+                 (r0,o0);(r1,o1);
+                 (r2,o2)] ++ R36)... }
       apply multi_step with
         (y:=((cur_stkh,SH_tup,SH_conts),
               [(ip,loc_w (incr_cloc 2 l));
                (sp,loc_w (hloc L_out (List.length cur_stk_val)));
-               (nat_reg 0,o0);
-               (nat_reg 1,nth i (List.map run_cst_trans lst0) ns);
-               (nat_reg 2,o2)] ++ R36)).
+               (r0,o0);
+               (r1,nth i (List.map run_cst_trans lst0) ns);
+               (r2,o2)] ++ R36)).
       { apply S_load_tup with
-          (d:=1) (s:=nat_reg 1) (off:=i)
+          (d:=r1) (s:=r1) (off:=i)
           (L:=L_str) (lst:=(List.map run_cst_trans lst0)) 
           (R:=[(ip,loc_w (next_cloc l));
                (sp,loc_w (hloc L_out (List.length cur_stk_val)));
-               (nat_reg 0,o0);
-               (nat_reg 1,val_direct_trans v cur_stk_val);
-               (nat_reg 2,o2)] ++ R36)...
-        - rewrite H15. inversion H11...
+               (r0,o0);
+               (r1,val_direct_trans v cur_stk_val);
+               (r2,o2)] ++ R36)...
+        - rewrite H15. inversion H10...
           apply ins_verify with (n:=1).
         - destruct v as [cst|[ind|str]]...
           inversion H4... rewrite app_nth1.
           rewrite map_nth with (d:=L.ns).
           rewrite H2... rewrite map_length.
-          inversion H17... inversion H7... inversion H3...
+          inversion H10... inversion H3... inversion H8...
+          inversion H6...
         - inversion H13... inversion H2... }
       constructor. 
       apply S_push with
-      (o:=reg_o (nat_reg 1)) 
-      (R:=[(ip,loc_w (incr_cloc 2 l));
-           (sp,loc_w (hloc L_out (List.length cur_stk_val)));
-           (nat_reg 0,o0);
-           (nat_reg 1,nth i (List.map run_cst_trans lst0) ns);
-           (nat_reg 2,o2)] ++ R36)...
-      rewrite H15. inversion H11. apply ins_verify with (n:=2).
+        (o:=r1) 
+        (R:=[(ip,loc_w (incr_cloc 2 l));
+             (sp,loc_w (hloc L_out (List.length cur_stk_val)));
+             (r0,o0);
+             (r1,nth i (List.map run_cst_trans lst0) ns);
+             (r2,o2)] ++ R36)...
+      rewrite H15. inversion H10. apply ins_verify with (n:=2).
     + (* prove LS_rel for L_get *)
       unfold incr_cloc...
       apply rel_LS with
         (lst:=lst ++ firstn 3 SIlst)
-        (SIlst:= tl (tl (tl SIlst)));inversion H11...
+        (SIlst:= tl (tl (tl SIlst)));inversion H10...
       * pose proof term_trans_not_nil as NN. specialize NN with
-        (tm:=t1'). destruct (RelConfig.LS.term_trans t1')as []eqn:?;automate.
+          (tm:=t1'). destruct (RelConfig.LS.term_trans t1')as []eqn:?;automate.
         rewrite <- Heql. rewrite <- PeanoNat.Nat.add_succ_comm.
-        apply rel_tm with (E:=nth i lst0 L.ns :: E1) (t:=t1').
+        apply rel_ins. inversion H2...
       * apply rel_env_context with (s_out:=s_out)...
         rewrite <- map_nth with (d:=L.ns)...
       * rewrite H15... assert (AssocIns: forall (x1:instr) x2 x3 tl,
-          [x1;x2;x3] ++ tl = x1::x2::x3::tl). { intros... }
+                                  [x1;x2;x3] ++ tl = x1::x2::x3::tl). { intros... }
         rewrite <- AssocIns,app_assoc...
       * rewrite app_length. rewrite PeanoNat.Nat.add_comm...
-      * destruct t1';inversion H17...
   - (* x = v1[i] <- v2 *)
     destruct L as [L_str].
     exists ((L_out,
@@ -501,77 +510,77 @@ Proof with super_a.
               :: H_stack,
              hloc_str L_str !->t
                tuple (update_nth 0 (List.map run_cst_trans [c])
-               (val_direct_trans v' cur_stk_val)); SH_tup,SH_conts),
+                        (val_direct_trans v' cur_stk_val)); SH_tup,SH_conts),
       ([(ip,loc_w (incr_cloc 4 l));
         (sp,loc_w (hloc L_out (1+(List.length cur_stk_val))));
-        (nat_reg 0,o0);
-        (nat_reg 1,val_direct_trans v' cur_stk_val);
-        (nat_reg 2,loc_w (hloc L_str 0))] ++ R36). split.
+        (r0,o0);
+        (r1,val_direct_trans v' cur_stk_val);
+        (r2,loc_w (hloc L_str 0))] ++ R36). split.
     (* stepping salt code for storing to heap *)
     + apply multi_step with
         (y:=((cur_stkh,SH_tup,SH_conts),
               [(ip,loc_w (next_cloc l));
                (sp,loc_w (hloc L_out (List.length cur_stk_val)));
-               (nat_reg 0,o0);
-               (nat_reg 1,val_direct_trans v' cur_stk_val);
-               (nat_reg 2,o2)] ++ R36)).
+               (r0,o0);
+               (r1,val_direct_trans v' cur_stk_val);
+               (r2,o2)] ++ R36)).
       { destruct v' as [cst|[ind|str]].
         - apply S_mov with
-            (d:=1) (o:=val_direct_trans (const_val cst) cur_stk_val)
+            (d:=r1) (o:=val_direct_trans (const_val cst) cur_stk_val)
             (R:=[(ip,loc_w l);(sp,loc_w (hloc L_out (List.length cur_stk_val)));
-                 (nat_reg 0,o0);(nat_reg 1,o1);
-                 (nat_reg 2,o2)] ++ R36)...
-          rewrite H15. inversion H11... apply nth_middle.
-        - pose proof S_load_stk as Ins. specialize Ins with
-            (d:=1) (s:=sp) (off:=ind)
-            (L:=L_out) (sign:=false)
+                 (r0,o0);(r1,o1);
+                 (r2,o2)] ++ R36)...
+          rewrite H15. inversion H10... apply nth_middle.
+        - pose proof S_load_sp as Ins. specialize Ins with
+            (d:=r1) (off:=ind)
+            (L:=L_out) 
             (lst:=cur_stk_val) (i:=List.length cur_stk_val)
             (R:=[(ip,loc_w l);(sp,loc_w (hloc L_out (List.length cur_stk_val)));
-                 (nat_reg 0,o0);(nat_reg 1,o1);
-                 (nat_reg 2,o2)] ++ R36).
+                 (r0,o0);(r1,o1);
+                 (r2,o2)] ++ R36).
           rewrite PeanoNat.Nat.sub_diag in Ins.
-          destruct SH_conts. apply Ins...
-          + inversion H11. rewrite H15... apply nth_middle.
+          apply Ins...
+          + inversion H10. rewrite H15... apply nth_middle.
           + rewrite h_eqb_refl...
         - apply S_mov with
-            (d:=1) (o:=val_direct_trans (var_val str) cur_stk_val)
+            (d:=r1) (o:=val_direct_trans (var_val str) cur_stk_val)
             (R:=[(ip,loc_w l);(sp,loc_w (hloc L_out (List.length cur_stk_val)));
-                 (nat_reg 0,o0);(nat_reg 1,o1);
-                 (nat_reg 2,o2)] ++ R36)...
-          rewrite H15. inversion H11... apply nth_middle. }
+                 (r0,o0);(r1,o1);
+                 (r2,o2)] ++ R36)...
+          rewrite H15. inversion H10... apply nth_middle. }
       apply multi_step with
         (y:=((cur_stkh,SH_tup,SH_conts),
               [(ip,loc_w (incr_cloc 2 l));
                (sp,loc_w (hloc L_out (List.length cur_stk_val)));
-               (nat_reg 0,o0);
-               (nat_reg 1,val_direct_trans v' cur_stk_val);
-               (nat_reg 2,loc_w (hloc L_str 0))] ++ R36)).
+               (r0,o0);
+               (r1,val_direct_trans v' cur_stk_val);
+               (r2,loc_w (hloc L_str 0))] ++ R36)).
       { destruct v as [cst|[ind|str]].
         - apply S_mov with
-            (d:=2) (o:=loc_w (hloc L_str 0))
+            (d:=r2) (o:=loc_w (hloc L_str 0))
             (R:=[(ip,loc_w (next_cloc l));(sp,loc_w (hloc L_out (List.length cur_stk_val)));
-                 (nat_reg 0,o0);
-                 (nat_reg 1,val_direct_trans v' cur_stk_val);
-                 (nat_reg 2,o2)] ++ R36)...
-        - pose proof S_load_stk as Ins. specialize Ins with
-            (d:=2) (s:=sp) (off:=ind) (l:=next_cloc l)
-            (L:=L_out) (sign:=false)
+                 (r0,o0);
+                 (r1,val_direct_trans v' cur_stk_val);
+                 (r2,o2)] ++ R36)...
+        - pose proof S_load_sp as Ins. specialize Ins with
+            (d:=r2) (off:=ind) (l:=next_cloc l)
+            (L:=L_out) 
             (lst:=cur_stk_val) (i:=List.length cur_stk_val)
             (R:=[(ip,loc_w (next_cloc l));
                  (sp,loc_w (hloc L_out (List.length cur_stk_val)));
-                 (nat_reg 0,o0);
-                 (nat_reg 1,val_direct_trans v' cur_stk_val);
-                 (nat_reg 2,o2)] ++ R36).
+                 (r0,o0);
+                 (r1,val_direct_trans v' cur_stk_val);
+                 (r2,o2)] ++ R36).
           rewrite PeanoNat.Nat.sub_diag in Ins.
           assert (Temp:loc_w (hloc L_str 0)
                        = nth (0 + ind) cur_stk_val ns).
           { inversion H8... rewrite app_nth1...
             rewrite map_nth with (d:=L.ns).
             rewrite H2... rewrite List.map_length...
-            inversion H17... inversion H6...
-            inversion H4... }
-          destruct SH_conts. rewrite Temp. apply Ins...
-          + inversion H11. rewrite H15... apply ins_verify with (n:=1).
+            inversion H10... inversion H3...
+            inversion H7... inversion H6... }
+          rewrite Temp. apply Ins...
+          + inversion H10. rewrite H15... apply ins_verify with (n:=1).
           + rewrite h_eqb_refl...
         - inversion H5... }
       apply multi_step with
@@ -582,295 +591,714 @@ Proof with super_a.
               SH_tup,SH_conts),
               [(ip,loc_w (incr_cloc 3 l));
                (sp,loc_w (hloc L_out (List.length cur_stk_val)));
-               (nat_reg 0,o0);
-               (nat_reg 1,val_direct_trans v' cur_stk_val);
-               (nat_reg 2,loc_w (hloc L_str 0))] ++ R36)).
+               (r0,o0);
+               (r1,val_direct_trans v' cur_stk_val);
+               (r2,loc_w (hloc L_str 0))] ++ R36)).
       { apply S_store with
-          (d:=2) (o:=reg_o 1) (j:=0) (L:=hloc_str L_str)
+          (d:=r2) (o:=r1) (j:=0) (L:=hloc_str L_str)
           (lst:=List.map run_cst_trans [c])
           (R:=[(ip,loc_w (incr_cloc 2 l));
                (sp,loc_w (hloc L_out (List.length cur_stk_val)));
-               (nat_reg 0,o0);
-               (nat_reg 1,val_direct_trans v' cur_stk_val);
-               (nat_reg 2,loc_w (hloc L_str 0))] ++ R36)...
-        - rewrite H15. inversion H19... inversion H11.
+               (r0,o0);
+               (r1,val_direct_trans v' cur_stk_val);
+               (r2,loc_w (hloc L_str 0))] ++ R36)...
+        - rewrite H15. inversion H18... inversion H10.
           apply ins_verify with (n:=2).
         - inversion H13... inversion H2...
           apply H1 with (vs:=[c])... }
       constructor.
       apply S_push with
-        (o:=reg_o (nat_reg 1)) 
+        (o:=r1) 
         (R:=[(ip,loc_w (incr_cloc 3 l));
              (sp,loc_w (hloc L_out (List.length cur_stk_val)));
-             (nat_reg 0,o0);
-             (nat_reg 1,val_direct_trans v' cur_stk_val);
-             (nat_reg 2,loc_w (hloc L_str 0))] ++ R36)...
-      rewrite H15. inversion H11. apply ins_verify with (n:=3).
+             (r0,o0);
+             (r1,val_direct_trans v' cur_stk_val);
+             (r2,loc_w (hloc L_str 0))] ++ R36)...
+      rewrite H15. inversion H10. apply ins_verify with (n:=3).
     + (* prove LS_rel for assignment *)
       unfold incr_cloc...
       apply rel_LS with
         (lst:=lst ++ firstn 4 SIlst)
-        (SIlst:= tl(tl (tl (tl SIlst))));inversion H11...
+        (SIlst:= tl(tl (tl (tl SIlst))));inversion H10...
       * pose proof term_trans_not_nil as NN. specialize NN with
-        (tm:=t1'). destruct (RelConfig.LS.term_trans t1')as []eqn:?;automate.
+          (tm:=t1'). destruct (RelConfig.LS.term_trans t1')as []eqn:?;automate.
         rewrite <- Heql. rewrite <- PeanoNat.Nat.add_succ_comm.
-        apply rel_tm with (E:=L.var_deref E1 v' :: E1) (t:=t1').
+        apply rel_ins. inversion H2...
       * apply rel_env_context with (s_out:=s_out)...
         destruct v'... destruct v0...
         rewrite <- map_nth with (d:=L.ns).
-        rewrite app_nth1... inversion H17...
-        inversion H4... rewrite map_length. inversion H9...
+        rewrite app_nth1... rewrite map_length.
+        inversion H2... inversion H6...
+        inversion H11...
       * unfold th_update,L.th_update,L.h_eqb,h_eqb.
-        inversion H19...
+        inversion H18...
         intros. destruct (String.eqb L_str L_tup)...
         -- inversion H1... destruct v' as [|[|]]...
            rewrite <- map_nth with (d:=L.ns)...
-           rewrite app_nth1... inversion H17... inversion H6...
-           rewrite List.map_length... inversion H10...
-        -- inversion H13... inversion H3...
+           rewrite app_nth1... inversion H2... inversion H7...
+           rewrite List.map_length... inversion H16...
+        -- inversion H13... inversion H4...
       * rewrite H15... assert (AssocIns: forall (x1:instr) x2 x3 x4 tl,
-          [x1;x2;x3;x4] ++ tl = x1::x2::x3::x4::tl). { intros... }
+                                  [x1;x2;x3;x4] ++ tl = x1::x2::x3::x4::tl). { intros... }
         rewrite <- AssocIns,app_assoc...
       * rewrite app_length. rewrite PeanoNat.Nat.add_comm...
-      * destruct t1';inversion H17...
-          
   - (* x = v(v') *)
     destruct lab as [lab].
     exists ((L_out,stack ((val_direct_trans v' cur_stk_val)::
                             (loc_w (incr_cloc 3 l)) :: cur_stk_val))
-                :: H_stack,SH_tup,SH_conts),
-         ([(ip,loc_w (cloc lab 1));
-           (sp,loc_w (hloc L_out (2 + (List.length cur_stk_val))));
-           (nat_reg 0,loc_w (cloc lab 0));
-           (nat_reg 1,val_direct_trans v' cur_stk_val);
-           (nat_reg 2,o2)] ++ R36). split.
+              :: H_stack,SH_tup,SH_conts),
+      ([(ip,loc_w (cloc lab 1));
+        (sp,loc_w (hloc L_out (2 + (List.length cur_stk_val))));
+        (r0,loc_w (cloc lab 0));
+        (r1,val_direct_trans v' cur_stk_val);
+        (r2,o2)] ++ R36). split.
     + apply multi_step with
         (y:=(cur_stkh,SH_tup,SH_conts,
               [(ip,loc_w (next_cloc l));
                (sp,loc_w (hloc L_out (List.length cur_stk_val)));
-               (nat_reg 0,loc_w (cloc lab 0));
-               (nat_reg 1,o1);(nat_reg 2,o2)] ++ R36)).
+               (r0,loc_w (cloc lab 0));
+               (r1,o1);(r2,o2)] ++ R36)).
       { destruct v as [cst|[ind|str]].
         - apply S_mov with
-            (d:=0) (o:=loc_w (cloc lab 0))
+            (d:=r0) (o:=loc_w (cloc lab 0))
             (R:=[(ip,loc_w l);
                  (sp,loc_w (hloc L_out (List.length cur_stk_val)));
-                 (nat_reg 0,o0);(nat_reg 1,o1);
-                 (nat_reg 2,o2)] ++ R36)...
-          rewrite H15. inversion H11... inversion H7...
+                 (r0,o0);(r1,o1);
+                 (r2,o2)] ++ R36)...
+          rewrite H15. inversion H10... inversion H7...
           apply nth_middle.
-        - pose proof S_load_stk as Ins. specialize Ins with
-            (d:=0) (s:=sp) (off:=ind)
-            (L:=L_out) (sign:=false)
+        - pose proof S_load_sp as Ins. specialize Ins with
+            (d:=r0) (off:=ind)
+            (L:=L_out) 
             (lst:=cur_stk_val) (i:=List.length cur_stk_val)
             (R:=[(ip,loc_w l);
                  (sp,loc_w (hloc L_out (List.length cur_stk_val)));
-                 (nat_reg 0,o0);(nat_reg 1,o1);
-                 (nat_reg 2,o2)] ++ R36).
+                 (r0,o0);(r1,o1);
+                 (r2,o2)] ++ R36).
           rewrite PeanoNat.Nat.sub_diag in Ins.
           assert (Temp:loc_w (cloc lab 0)
                        = nth (0 + ind) cur_stk_val ns).
           { inversion H7... rewrite app_nth1...
             rewrite map_nth with (d:=L.ns).
             rewrite H2... rewrite List.map_length...
-            inversion H17... inversion H6... inversion H9... }
-          destruct SH_conts. rewrite Temp. apply Ins...
-          + inversion H11. rewrite H15... apply nth_middle.
+            inversion H10... inversion H3... inversion H8...
+            inversion H11... }
+          rewrite Temp. apply Ins...
+          + inversion H10. rewrite H15... apply nth_middle.
           + rewrite h_eqb_refl...
         - inversion H7... }
       apply multi_step with
         (y:=(cur_stkh,SH_tup,SH_conts,
               [(ip,loc_w (incr_cloc 2 l));
                (sp,loc_w (hloc L_out (List.length cur_stk_val)));
-               (nat_reg 0,loc_w (cloc lab 0));
-               (nat_reg 1,val_direct_trans v' cur_stk_val);
-               (nat_reg 2,o2)] ++ R36)).
+               (r0,loc_w (cloc lab 0));
+               (r1,val_direct_trans v' cur_stk_val);
+               (r2,o2)] ++ R36)).
       { destruct v' as [cst|[ind|str]].
         - apply S_mov with
-            (d:=1) (o:=val_direct_trans (const_val cst) cur_stk_val)
+            (d:=r1) (o:=val_direct_trans (const_val cst) cur_stk_val)
             (R:=[(ip,loc_w (next_cloc l));
                  (sp,loc_w (hloc L_out (List.length cur_stk_val)));
-                 (nat_reg 0,loc_w (cloc lab 0));
-                 (nat_reg 1,o1);(nat_reg 2,o2)] ++ R36)...
-          rewrite H15. inversion H11... inversion H7...
+                 (r0,loc_w (cloc lab 0));
+                 (r1,o1);(r2,o2)] ++ R36)...
+          rewrite H15. inversion H10... inversion H7...
           apply ins_verify with (n:=1).
-        - pose proof S_load_stk as Ins. specialize Ins with
-            (d:=1) (s:=sp) (off:=ind)
-            (L:=L_out) (sign:=false)
+        - pose proof S_load_sp as Ins. specialize Ins with
+            (d:=r1) (off:=ind)
+            (L:=L_out) 
             (lst:=cur_stk_val) (i:=List.length cur_stk_val)
             (R:=[(ip,loc_w (next_cloc l));
                  (sp,loc_w (hloc L_out (List.length cur_stk_val)));
-                 (nat_reg 0,loc_w (cloc lab 0));
-                 (nat_reg 1,o1);(nat_reg 2,o2)] ++ R36).
+                 (r0,loc_w (cloc lab 0));
+                 (r1,o1);(r2,o2)] ++ R36).
           rewrite PeanoNat.Nat.sub_diag in Ins.
-          destruct SH_conts. apply Ins...
-          + inversion H11. rewrite H15... apply ins_verify with (n:=1).
+          apply Ins...
+          + inversion H10. rewrite H15... apply ins_verify with (n:=1).
           + rewrite h_eqb_refl...
         - apply S_mov with
-            (d:=1) (o:=val_direct_trans (var_val str) cur_stk_val)
+            (d:=r1) (o:=val_direct_trans (var_val str) cur_stk_val)
             (R:=[(ip,loc_w (next_cloc l));
                  (sp,loc_w (hloc L_out (List.length cur_stk_val)));
-                 (nat_reg 0,loc_w (cloc lab 0));
-                 (nat_reg 1,o1);(nat_reg 2,o2)] ++ R36)...
-          rewrite H15. inversion H11... inversion H7...
+                 (r0,loc_w (cloc lab 0));
+                 (r1,o1);(r2,o2)] ++ R36)...
+          rewrite H15. inversion H10... inversion H7...
           apply ins_verify with (n:=1). }
       apply multi_step with
         (y:=((L_out, stack (loc_w (incr_cloc 3 l) :: cur_stk_val)) :: H_stack,
-           SH_tup, SH_conts,
-           [(ip,loc_w (cloc lab 0));
-            (sp,loc_w (hloc L_out (1 + List.length cur_stk_val)));
-            (nat_reg 0,loc_w (cloc lab 0));
-            (nat_reg 1,val_direct_trans v' cur_stk_val);
-            (nat_reg 2,o2)] ++ R36)).
+              SH_tup, SH_conts,
+              [(ip,loc_w (cloc lab 0));
+               (sp,loc_w (hloc L_out (1 + List.length cur_stk_val)));
+               (r0,loc_w (cloc lab 0));
+               (r1,val_direct_trans v' cur_stk_val);
+               (r2,o2)] ++ R36)).
       { apply S_call with
-        (o:=reg_o (nat_reg 0))
-        (R:=[(ip,loc_w (incr_cloc 2 l));
-             (sp,loc_w (hloc L_out (List.length cur_stk_val)));
-             (nat_reg 0,loc_w (cloc lab 0));
-             (nat_reg 1,val_direct_trans v' cur_stk_val);
-             (nat_reg 2,o2)] ++ R36)...
-        rewrite H15. inversion H11...
+          (o:=r0)
+          (R:=[(ip,loc_w (incr_cloc 2 l));
+               (sp,loc_w (hloc L_out (List.length cur_stk_val)));
+               (r0,loc_w (cloc lab 0));
+               (r1,val_direct_trans v' cur_stk_val);
+               (r2,o2)] ++ R36)...
+        rewrite H15. inversion H10...
         apply ins_verify with (n:=2). }
       constructor.
       apply S_push with
-        (o:=reg_o (nat_reg 1)) (lst:=loc_w (incr_cloc 3 l) :: cur_stk_val)
+        (o:=r1) (lst:=loc_w (incr_cloc 3 l) :: cur_stk_val)
         (l:=cloc lab 0)
         (R:=[(ip,loc_w (cloc lab 0));
              (sp,loc_w (hloc L_out (1 + (List.length cur_stk_val))));
-             (nat_reg 0,loc_w (cloc lab 0));
-             (nat_reg 1,val_direct_trans v' cur_stk_val);
-             (nat_reg 2,o2)] ++ R36)...
-      inversion H14;super_a;rewrite H19...
+             (r0,loc_w (cloc lab 0));
+             (r1,val_direct_trans v' cur_stk_val);
+             (r2,o2)] ++ R36)...
+      inversion H14... inversion H18.
+      apply H3 in H18. unfold c_comp.
+      rewrite H18... rewrite H4...
     + (* prove LS_rel for v(v') *)
-      unfold incr_cloc,next_cloc... destruct (SC lab) as [newIns].
+      unfold incr_cloc,next_cloc... destruct (SC0 lab) as [newIns|]eqn:?.
       apply rel_LS with
-        (lst:=[push (reg_o 1)]) (SIlst:=func_term_trans 1 t1');
-        inversion H11;automate.
+        (lst:=[push r1]) (SIlst:=func_term_trans 1 t1');
+        inversion H10;automate.
+      * inversion H14... specialize H3 with (c_lab lab).
+        rewrite H18 in H3. inversion H3... 
       * apply rel_env_context with
-          (s_out:=loc_w (cloc Clab (3 + (Datatypes.length lst)))
+          (s_out:=loc_w (cloc Clab (3 + (List.length lst)))
                     :: List.map run_cst_trans E1 ++ s_out).
         { inversion H5...
           - intros. inversion H1...
             assert (Temp:stk_points_to s_out s' L').
-            { apply H2 with (L:=L) (H':=H')... }
+            { apply H3 with (L:=L) (H':=H')... }
             unfold stk_points_to in Temp.
             unfold stk_points_to. rewrite <- Temp.
             rewrite app_comm_cons. rewrite rev_app_distr.
             apply nth_error_app1. apply nth_error_Some.
             rewrite Temp. unfold not. intros...
-          - inversion H3... rewrite app_comm_cons.
+          - inversion H4... rewrite app_comm_cons.
             apply rel_hdl_stk_lst... rewrite app_comm_cons.
-            inversion H16...
+            inversion H17...
             + repeat (rewrite app_comm_cons).
               rewrite app_assoc.
               apply rel_hdl_stk_base with
                 (frm:=frm) (frm_stk:=frm_stk)...
               rewrite app_comm_cons. constructor...
               apply rel_frame with
-                (C_mem:=SC)
-                (lst:=lst ++ [val_trans 0 v;val_trans 1 v';
-                              call (reg_o 0)])
-                (Ilst:=push (reg_o 1) :: func_term_trans (S (List.length E1)) t)...
-              rewrite H15. cbn. pose proof term_trans_not_nil as NN.
-              specialize NN with (tm:=t).
-              destruct (term_trans t) as []eqn:?;automate.
-              rewrite <- Heql. unfold func_term_trans.
-              rewrite <- PeanoNat.Nat.add_succ_comm.
-              rewrite <- app_assoc...
-              rewrite app_length... rewrite PeanoNat.Nat.add_comm...
+                (C_mem:=c_comp S_builtin_ins SC0)
+                (lst:=lst ++ [val_trans r0 v;val_trans r1 v';
+                              call r0])
+                (Ilst:=push r1 :: func_term_trans (S (List.length E1)) t)...
+              * inversion H2...
+              * rewrite H15. cbn. pose proof term_trans_not_nil as NN.
+                specialize NN with (tm:=t).
+                destruct (term_trans t) as []eqn:?;automate.
+                rewrite <- Heql. unfold func_term_trans.
+                rewrite <- PeanoNat.Nat.add_succ_comm.
+                rewrite <- app_assoc...
+              * rewrite app_length... rewrite PeanoNat.Nat.add_comm...
             + repeat (rewrite app_comm_cons).
               rewrite app_assoc.
               apply rel_hdl_stk with
                 (frm:=frm) (frm_stk:=frm_stk)...
               rewrite app_comm_cons. constructor...
               apply rel_frame with
-                (C_mem:=SC)
-                (lst:=lst ++ [val_trans 0 v;val_trans 1 v';
-                              call (reg_o 0)])
-                (Ilst:=push (reg_o 1) :: func_term_trans (S (List.length E1)) t)...
-              rewrite H15. cbn. pose proof term_trans_not_nil as NN.
-              specialize NN with (tm:=t).
-              destruct (term_trans t) as []eqn:?;automate.
-              rewrite <- Heql. unfold func_term_trans.
-              rewrite <- PeanoNat.Nat.add_succ_comm.
-              rewrite <- app_assoc...
-              rewrite app_length... rewrite PeanoNat.Nat.add_comm... }
+                (C_mem:=c_comp S_builtin_ins SC0)
+                (lst:=lst ++ [val_trans r0 v;val_trans r1 v';
+                              call r0])
+                (Ilst:=push r1 :: func_term_trans (S (List.length E1)) t)...
+              * inversion H2...
+              * rewrite H15. cbn. pose proof term_trans_not_nil as NN.
+                specialize NN with (tm:=t).
+                destruct (term_trans t) as []eqn:?;automate.
+                rewrite <- Heql. unfold func_term_trans.
+                rewrite <- PeanoNat.Nat.add_succ_comm.
+                rewrite <- app_assoc...
+              * rewrite app_length... rewrite PeanoNat.Nat.add_comm... }
         destruct v' as [cst|[ind|str]]...
         rewrite <- map_nth with (d:=L.ns). rewrite app_nth1...
-        inversion H17... rewrite List.map_length... inversion H4...
-        assert (Temp:wf_val (Datatypes.length E1) (var_val ind)).
-        { apply H3... } inversion Temp...           
-      * inversion H14... rewrite H19...
-      * inversion H14... specialize H2 with (c_lab lab).
-        unfold wf_func_tm in H2. rewrite H19 in H2.
-        inversion H2... 
+        inversion H2... rewrite List.map_length...
+        inversion H6...
+        specialize H4 with (v':=L.var_val ind).
+        assert (Temp:In (L.var_val ind) [L.var_val (L.dbjind_var ind)]).
+        { super_a. } apply H4 in Temp. inversion Temp...
+      * inversion H14... inversion H18.
+        apply H4 in H6. unfold c_comp.
+        rewrite H6. unfold code_mem_trans.
+        rewrite H18...
+      * inversion H14... unfold code_mem_trans in Heqi.
+        rewrite H18 in Heqi...
   - (* v end, return from function call *)
     (* move result to r1, chop stack via sfree
        (sp's label and Lsp changes accordingly)
      then return (ip changes, stack further chops *)
     exists ((L_out,stack (val_direct_trans v cur_stk_val :: (tl s_out)))
               :: H_stack,SH_tup,SH_conts),
-    ([(ip,nth 0 s_out ns);
-      (sp,loc_w (hloc L_out (List.length s_out))); (*remove l_dst, add v*)
-      (nat_reg 0,o0);
-      (nat_reg 1,val_direct_trans v cur_stk_val);(nat_reg 2,o2)] ++ R36).
+      ([(ip,match nth 0 s_out ns with
+            | cloc Clab n => cloc Clab (S n)
+            | _ => ns_cloc end);
+        (sp,loc_w (hloc L_out (List.length s_out))); (*remove l_dst, add v*)
+        (r0,o0);
+        (r1,val_direct_trans v cur_stk_val);(r2,o2)] ++ R36).
     split.
     apply multi_step with
       (y:=((cur_stkh,SH_tup,SH_conts),
             [(ip,loc_w (next_cloc l));
              (sp,loc_w (hloc L_out (List.length cur_stk_val)));
-             (nat_reg 0,o0);
-             (nat_reg 1,val_direct_trans v cur_stk_val);
-             (nat_reg 2,o2)] ++ R36)).
+             (r0,o0);
+             (r1,val_direct_trans v cur_stk_val);
+             (r2,o2)] ++ R36)).
     { destruct v as [cst|[ind|str]].
       - apply S_mov with
-          (d:=1) (o:=val_direct_trans (const_val cst) cur_stk_val)
+          (d:=r1) (o:=val_direct_trans (const_val cst) cur_stk_val)
           (R:=[(ip,loc_w l);
                (sp,loc_w (hloc L_out (List.length cur_stk_val)));
-               (nat_reg 0,o0);(nat_reg 1,o1);
-               (nat_reg 2,o2)] ++ R36)...
-        inversion H11... rewrite H15... apply nth_middle.
-      - pose proof S_load_stk as Ins. specialize Ins with
-          (d:=1) (s:=sp) (off:=ind)
-          (L:=L_out) (sign:=false)
+               (r0,o0);(r1,o1);
+               (r2,o2)] ++ R36)...
+        inversion H10... rewrite H15... apply nth_middle.
+      - pose proof S_load_sp as Ins. specialize Ins with
+          (d:=r1) (off:=ind)
+          (L:=L_out)
           (lst:=cur_stk_val) (i:=List.length cur_stk_val)
           (R:=[(ip,loc_w l);
                (sp,loc_w (hloc L_out (List.length cur_stk_val)));
-               (nat_reg 0,o0);(nat_reg 1,o1);
-               (nat_reg 2,o2)] ++ R36).
+               (r0,o0);(r1,o1);
+               (r2,o2)] ++ R36).
         rewrite PeanoNat.Nat.sub_diag in Ins.
-        destruct SH_conts. apply Ins...
-        + inversion H11. rewrite H15... apply nth_middle.
+        apply Ins...
+        + inversion H10. rewrite H15... apply nth_middle.
         + rewrite h_eqb_refl...
       - apply S_mov with
-          (d:=1) (o:=val_direct_trans (var_val str) cur_stk_val)
+          (d:=r1) (o:=val_direct_trans (var_val str) cur_stk_val)
           (R:=[(ip,loc_w l);
                (sp,loc_w (hloc L_out (List.length cur_stk_val)));
-               (nat_reg 0,o0);(nat_reg 1,o1);
-               (nat_reg 2,o2)] ++ R36)...
-        inversion H11... rewrite H15... apply nth_middle. }
+               (r0,o0);(r1,o1);
+               (r2,o2)] ++ R36)...
+        inversion H10... rewrite H15... apply nth_middle. }
     apply multi_step with
       (y:=((L_out,stack s_out) :: H_stack,SH_tup,SH_conts,
             [(ip,loc_w (incr_cloc 2 l));
              (sp,loc_w (hloc L_out (List.length s_out)));
-             (nat_reg 0,o0);
-             (nat_reg 1,val_direct_trans v cur_stk_val);
-             (nat_reg 2,o2)] ++ R36)).
-    { lemma on cdr_nth
-      assert (cdr_nth (Datatypes.length E1) cur_stk_val) =  s_out.
-      assert ((List.length - Datatypes.length E1) = length s_out
-      apply S_sfree with
-        (n:=List.length E1)
+             (r0,o0);
+             (r1,val_direct_trans v cur_stk_val);
+             (r2,o2)] ++ R36)).
+    { assert (Temp:skipn (List.length E1) cur_stk_val = s_out).
+      { cbn... rewrite skipn_app, skipn_map, skipn_all...
+        rewrite map_length, PeanoNat.Nat.sub_diag... }
+      assert (Temp2:List.length cur_stk_val - List.length E1 = List.length s_out).
+      { cbn... rewrite app_length, PeanoNat.Nat.add_comm,
+          map_length. apply PeanoNat.Nat.add_sub. }
+       pose proof S_sfree as Hyp. specialize Hyp with
+        (n:=List.length E1) (lst:=cur_stk_val)
         (R:=[(ip,loc_w (next_cloc l));
              (sp,loc_w (hloc L_out (List.length cur_stk_val)));
-             (nat_reg 0,o0);
-             (nat_reg 1,val_direct_trans v cur_stk_val);
-             (nat_reg 2,o2)] ++ R36)...
+             (r0,o0);
+             (r1,val_direct_trans v cur_stk_val);
+             (r2,o2)] ++ R36).
+      rewrite Temp in Hyp. rewrite <- Temp2.
+      apply Hyp...
+      - rewrite H15. inversion H10...
+        destruct v as [cst|[ind|str]];
+          rewrite PeanoNat.Nat.add_comm;
+          apply ins_verify with (n:=1).
+      - rewrite app_length, PeanoNat.Nat.add_comm.
+        destruct s_out;rewrite map_length...
+        apply PeanoNat.Nat.le_add_l. }
+    
+    apply multi_step with
+      (y:=((L_out,stack (tl s_out)) :: H_stack,SH_tup,SH_conts,
+            [(ip,hd ns s_out);
+             (sp,loc_w (hloc L_out (List.length (tl s_out))));
+             (r0,o0);
+             (r1,val_direct_trans v cur_stk_val);
+             (r2,o2)] ++ R36)).
+    { inversion H5... inversion H3...
+      pose proof S_ret as Hyp. specialize Hyp with
+        (l:=cloc Clab (2 + (List.length lst))).
+      remember (fun (s_prev:list word) (lst0:list instr) C_lab =>
+                   [(ip,loc_w (cloc Clab (2 + (List.length lst))));
+                    (sp,loc_w (hloc L_out (S (List.length s_prev))));
+                    (r0,o0);
+                    (r1,
+                      val_direct_trans v
+                        (List.map run_cst_trans E1 ++
+                           loc_w (cloc C_lab (List.length lst0)) :: s_prev));
+                    (r2,o2);(r3,o3);
+                    (r4,o4);(r5,o5);(r6,o6)])
+        as newR.
+      revert HeqnewR.
+      inversion H11... 
+      - inversion H1... inversion H16...
+        remember ((s ++ s') ++ frm_stk) as s_prev.
+        intros.
+        specialize Hyp with
+          (j:=S (List.length s_prev))
+          (l':=cloc C_lab (List.length lst0))
+          (R:=newR s_prev lst0 C_lab)...
+        cbn in Hyp. rewrite PeanoNat.Nat.sub_0_r in Hyp.
+        apply Hyp... rewrite H15. inversion H10...
+        destruct v as [|[|]];rewrite PeanoNat.Nat.add_comm;
+          apply ins_verify with (n:=2).
+      - inversion H6... inversion H17...
+        remember ((s ++ s') ++ frm_stk ++ slst) as s_prev.
+        intros.
+        specialize Hyp with
+          (j:=S (List.length s_prev))
+          (l':=cloc C_lab (List.length lst0))
+          (R:=newR s_prev lst0 C_lab)...
+        cbn in Hyp. rewrite PeanoNat.Nat.sub_0_r in Hyp.
+        apply Hyp... rewrite H15. inversion H10...
+        destruct v as [|[|]];rewrite PeanoNat.Nat.add_comm;
+          apply ins_verify with (n:=2). }
+    constructor.
+    { pose proof S_push as Hyp. specialize Hyp with
+        (o:=reg_o r1) (j:=List.length (tl s_out))
+        (*l:=cloc C_lab (List.length lst0)*)
+        (R:=[(ip,hd ns s_out);
+             (sp,loc_w (hloc L_out (List.length (tl s_out))));
+             (r0, o0);
+             (r1, val_direct_trans v cur_stk_val);
+             (r2, o2)] ++ R36).
+      inversion H5... inversion H3... inversion H11...
+      - inversion H1... inversion H16...
+        specialize Hyp with (l:=cloc C_lab (List.length lst0)).
+        cbn in Hyp. apply Hyp...
+        rewrite H19.
+        pose proof app_nth2_plus as Temp.
+        specialize Temp with (l:=lst0) (l':=Ilst) (n:=0).
+        rewrite PeanoNat.Nat.add_comm in Temp.
+        rewrite Temp...
+      - inversion H6... inversion H17...
+        specialize Hyp with (l:=cloc C_lab (List.length lst0)).
+        cbn in Hyp. apply Hyp...
+        rewrite H20.
+        pose proof app_nth2_plus as Temp.
+        specialize Temp with (l:=lst0) (l':=Ilst) (n:=0).
+        rewrite PeanoNat.Nat.add_comm in Temp.
+        rewrite Temp... }
+    + (* prove LS_rel for v end, end of function call *)
+      unfold incr_cloc,next_cloc,ns_cloc...
+      inversion H5... inversion H3...
+      inversion H11...
+      { inversion H1... inversion H16...
+         inversion H4...
+         apply rel_LS with
+           (lst:=lst0 ++ [nth 0 Ilst halt])
+           (SIlst:=tl Ilst)...
+        - inversion H17...
+        - apply rel_env_context with
+            (s_out:=s' ++ frm_stk)...
+          + intros. inversion H9...
+            assert (stk_points_to
+                      (loc_w (cloc C_lab (List.length lst0))
+                         :: s ++ s' ++ frm_stk)
+                      s'0 L').
+            { apply H2 with (L:=L) (H':=H').
+              repeat (rewrite <- app_assoc)... }
+            unfold stk_points_to. unfold stk_points_to in H20.
+            rewrite <- H20. rewrite app_comm_cons.
+            rewrite rev_app_distr with (y:=s'++frm_stk).
+            rewrite nth_error_app1...
+            rewrite rev_length. rewrite app_length.
+            rewrite PeanoNat.Nat.add_comm.
+            inversion H6;cbn;apply PeanoNat.Nat.lt_add_pos_r with (m:=3);
+              apply PeanoNat.Nat.lt_0_succ.
+          + inversion H21... rewrite app_assoc. 
+            destruct v as [cst|[ind|str]]...
+            rewrite <- map_nth with (d:=L.ns). rewrite app_nth1...
+            inversion H10... rewrite List.map_length... inversion H20...
+            inversion H24...
+        - rewrite H19... destruct Ilst... rewrite <- app_assoc...
+        - rewrite H23, app_length, PeanoNat.Nat.add_comm... } 
+      { inversion H6... inversion H17...
+        inversion H4...
+        apply rel_LS with
+          (lst:=lst0 ++ [nth 0 Ilst halt])
+          (SIlst:=tl Ilst)...
+        - inversion H18...
+        - apply rel_env_context with
+            (s_out:=s' ++ frm_stk ++ slst)...
+          + intros. inversion H16...
+            assert (stk_points_to
+                      (loc_w (cloc C_lab (List.length lst0))
+                         :: s ++ s' ++ frm_stk ++ slst)
+                      s'0 L').
+            { apply H2 with (L:=L) (H':=H').
+              repeat (rewrite <- app_assoc)... }
+            unfold stk_points_to. unfold stk_points_to in H21.
+            rewrite <- H21. rewrite app_comm_cons.
+            rewrite rev_app_distr with (y:=s'++frm_stk++slst).
+            rewrite nth_error_app1...
+            rewrite rev_length. repeat (rewrite app_length).
+            rewrite PeanoNat.Nat.add_comm.
+            inversion H7;cbn;apply PeanoNat.Nat.lt_add_pos_r with (m:=3);
+              apply PeanoNat.Nat.lt_0_succ.
+          + inversion H22... repeat (rewrite app_assoc). 
+            destruct v as [cst|[ind|str]]...
+            rewrite <- map_nth with (d:=L.ns). rewrite app_nth1...
+            inversion H10... rewrite List.map_length... inversion H21...
+            inversion H25...
+        - rewrite H20. destruct Ilst... rewrite <- app_assoc...
+        - rewrite H24, app_length, PeanoNat.Nat.add_comm... }
+  - (* handle P_body with A P_op under v_env in t*)
+    destruct lab_op as [lab_op],lab_body as [lab_body],
+          L as [L],(a_eqb general A) as [|]eqn:?.
+    (* split cases for types of handlers *)
+    *** assert (A = general). { destruct A... }
+        exists
+          ((hloc_str L,
+             stack
+               [val_direct_trans v_env cur_stk_val;
+                loc_w (hloc L 4);loc_w (cloc handle_loc 10);
+                loc_w (hloc L_out (S (List.length cur_stk_val)));
+                int_w 0;
+                val_direct_trans v_env cur_stk_val; 
+                loc_w (cloc (cloc_str lab_op) 0)])
+             :: (L_out, stack (loc_w (incr_cloc 5 l) :: cur_stk_val))
+             :: H_stack, SH_tup, SH_conts),
+          ([(ip,loc_w (cloc lab_body 2));
+            (sp,loc_w (hloc L 7));(r0, o0);
+            (r1,val_direct_trans v_env cur_stk_val);
+            (r2,loc_w (hloc L 4));
+            (r3,val_direct_trans v_env cur_stk_val);
+            (r4,int_w 0);
+            (r5,loc_w (hloc L_out (S (List.length cur_stk_val))));
+            (r6,loc_w (cloc lab_body 0))]). split.
+    + rewrite HeqR36. eapply multi_step.
+      { eapply S_mov with (d:=r4) (o:=0)...
+        inversion H10... rewrite H15...
+        apply nth_middle. }
+      eapply multi_step.
+      { destruct v_env as [|[|]].
+        - eapply S_mov with
+            (d:=r3) (o:=val_direct_trans s cur_stk_val)...
+        - pose proof S_load_sp as Temp.
+          specialize Temp with
+            (d:=r3) (off:=n) (lst:=cur_stk_val)
+            (i:=List.length cur_stk_val).
+          rewrite PeanoNat.Nat.sub_diag in Temp.
+          eapply Temp...
+          + rewrite H15. inversion H10...
+            apply ins_verify with (n:=1).
+          + rewrite h_eqb_refl...
+        - eapply S_mov with
+            (d:=r3) (o:=val_direct_trans (var_val v) cur_stk_val)... }
+      eapply multi_step.
+      { eapply S_mov with
+          (d:=r2) (o:=wd_o (cloc lab_op 0))...
+        inversion H10... rewrite H15...
+        apply ins_verify with (n:=2). }
+      eapply multi_step.
+      { eapply S_mov with
+          (d:=r1) (o:=wd_o (cloc lab_body 0))...
+        inversion H10... rewrite H15...
+        apply ins_verify with (n:=3). }
+      eapply multi_step.
+      { eapply S_call with
+          (o:=wd_o (cloc handle_loc 0))...
+        inversion H10... rewrite H15...
+        apply ins_verify with (n:=4). }
+      eapply multi_step.
+      { eapply S_mov with
+          (d:=r5) (o:=sp)... }
+      eapply multi_step.
+      { eapply S_mkstk with
+          (reg:=sp) (L:=L)... }
+      eapply multi_step.
+      { eapply S_push with (o:=r2)... }
+      eapply multi_step.
+      { eapply S_push with (o:=r3)... }
+      eapply multi_step.
+      { eapply S_push with (o:=r4)... }
+      eapply multi_step.
+      { eapply S_push with (o:=r5)... }
+      eapply multi_step.
+      { eapply S_mov with
+          (d:=r6) (o:=r1)... }
+      eapply multi_step.
+      { eapply S_mov with
+          (d:=r2) (o:=sp)... }
+      eapply multi_step.
+      { eapply S_mov with
+          (d:=r1) (o:=r3)... }
+      eapply multi_step.
+      { eapply S_call with (o:=r6)... }
+      eapply multi_step.
+      { eapply S_push with (o:=r2)...
+        unfold c_comp. inversion H14...
+        inversion H18... apply H3 in H4.
+        rewrite H4,H18... }
+      constructor.
+      { cbn. repeat (rewrite <- Heqcur_stk_val).
+        pose proof S_push as Temp.
+        specialize Temp with
+          (o:=reg_o r1) (l:=cloc lab_body 1)
+          (lst:=[loc_w (hloc L 4);
+                 loc_w (cloc handle_loc 10);
+                 loc_w (hloc L_out (S (Datatypes.length cur_stk_val)));
+                 int_w 0; val_direct_trans v_env cur_stk_val;
+                 loc_w (cloc lab_op 0)])
+          (R:=[(ip,loc_w (cloc lab_body 1));
+               (sp,loc_w (hloc L 6)); (r0, o0);
+               (r1,val_direct_trans v_env cur_stk_val);
+               (r2,loc_w (hloc L 4));
+               (r3,val_direct_trans v_env cur_stk_val);
+               (r4,int_w 0);
+               (r5,loc_w (hloc L_out (S (List.length cur_stk_val))));
+               (r6,loc_w (cloc lab_body 0))]).
+        cbn in Temp. apply Temp...
+        unfold c_comp. inversion H14...
+        inversion H18... apply H3 in H4.
+        rewrite H4,H18... }
+    + (* prove LS_rel for handler creation*)
+      unfold incr_cloc,next_cloc... destruct (SC0 lab_body) as [newIns|]eqn:?.
+      eapply rel_LS...
+      * inversion H14... specialize H2 with (c_lab lab_body).
+        rewrite H18 in H2. inversion H2... 
+      * apply rel_env_context with
+          (s_out:=
+             [loc_w (cloc handle_loc 10);
+              loc_w (hloc L_out
+                       (S (List.length (List.map run_cst_trans E1 ++ s_out))));
+              int_w 0; val_direct_trans v_env (List.map run_cst_trans E1 ++ s_out);
+              loc_w (cloc lab_op 0)])...
+        -- intros. inversion H1...
+        -- inversion H5...
 
-    4: { destruct (List.length l0). apply PeanoNat.Nat.lt_irrefl in H19;
-         destruct H19. 
-   
 
+wrong here already
+
+
+
+
+
+
+
+           apply rel_hdl_stk_lst with
+             (K:=[L.h_f (L.handler_f (L.hdl_lab L)
+                           L_env (L.c_lab lab_op) general)])...
+           { inversion H3... rewrite app_comm_cons.
+             apply rel_hdl_stk_lst... inversion H16;automate;
+               repeat (rewrite app_comm_cons).
+             - repeat (rewrite app_assoc).
+               apply rel_hdl_stk_base... rewrite app_comm_cons.
+               apply rel_frame_cons... apply rel_frame with
+                 (lst:=lst ++ firstn 5 SIlst) (Ilst:=skipn 5 SIlst);
+                 inversion H10;automate.
+               + pose proof term_trans_not_nil...
+                 destruct (term_trans t) as []eqn:?;automate.
+                 rewrite <- Heql.
+                 rewrite <- PeanoNat.Nat.add_succ_comm.
+                 apply rel_ins. inversion H11...
+               + rewrite H15...
+                 rewrite <- app_assoc...
+               + rewrite app_length...
+                 rewrite PeanoNat.Nat.add_comm...
+             - rewrite app_assoc with (m:=s). apply rel_hdl_stk...
+               rewrite app_comm_cons.
+               apply rel_frame_cons... apply rel_frame with
+                 (lst:=lst ++ firstn 5 SIlst) (Ilst:=skipn 5 SIlst);
+                 inversion H10;automate.
+               + pose proof term_trans_not_nil...
+                 destruct (term_trans t) as []eqn:?;automate.
+                 rewrite <- Heql.
+                 rewrite <- PeanoNat.Nat.add_succ_comm.
+                 apply rel_ins. inversion H17...
+               + rewrite H15...
+                 rewrite <- app_assoc...
+               + rewrite app_length...
+                 rewrite PeanoNat.Nat.add_comm... }
+           { apply rel_hdl_stk_base
+               with (Flst:=[]) (s:=[])... destruct L_env.
+             apply rel_hdl_general... rewrite app_comm_cons.
+               apply rel_frame_cons... apply rel_frame with
+                 (lst:=lst ++ firstn 5 SIlst) (Ilst:=skipn 5 SIlst);
+                 inversion H10;automate.
+               + pose proof term_trans_not_nil...
+                 destruct (term_trans t) as []eqn:?;automate.
+                 rewrite <- Heql.
+                 rewrite <- PeanoNat.Nat.add_succ_comm.
+                 apply rel_ins. inversion H11...
+               + rewrite H15...
+                 rewrite <- app_assoc...
+               + rewrite app_length...
+                 rewrite PeanoNat.Nat.add_comm...
+             - rewrite app_assoc with (m:=s). apply rel_hdl_stk...
+               rewrite app_comm_cons.
+               apply rel_frame_cons... apply rel_frame with
+                 (lst:=lst ++ firstn 5 SIlst) (Ilst:=skipn 5 SIlst);
+                 inversion H10;automate.
+               + pose proof term_trans_not_nil...
+                 destruct (term_trans t) as []eqn:?;automate.
+                 rewrite <- Heql.
+                 rewrite <- PeanoNat.Nat.add_succ_comm.
+                 apply rel_ins. inversion H17...
+               + rewrite H15...
+                 rewrite <- app_assoc...
+               + rewrite app_length...
+                 rewrite PeanoNat.Nat.add_comm... }
+
+
+
+
+
+           
+                 { inversion H5...
+          - intros. inversion H1...
+            assert (Temp:stk_points_to s_out s' L').
+            { apply H3 with (L:=L) (H':=H')... }
+            unfold stk_points_to in Temp.
+            unfold stk_points_to. rewrite <- Temp.
+            rewrite app_comm_cons. rewrite rev_app_distr.
+            apply nth_error_app1. apply nth_error_Some.
+            rewrite Temp. unfold not. intros...
+          - inversion H4... rewrite app_comm_cons.
+            apply rel_hdl_stk_lst... rewrite app_comm_cons.
+            inversion H17...
+            + repeat (rewrite app_comm_cons).
+              rewrite app_assoc.
+              apply rel_hdl_stk_base with
+                (frm:=frm) (frm_stk:=frm_stk)...
+              rewrite app_comm_cons. constructor...
+              apply rel_frame with
+                (C_mem:=c_comp S_builtin_ins SC0)
+                (lst:=lst ++ [val_trans r0 v;val_trans r1 v';
+                              call r0])
+                (Ilst:=push r1 :: func_term_trans (S (List.length E1)) t)...
+              * inversion H2...
+              * rewrite H15. cbn. pose proof term_trans_not_nil as NN.
+                specialize NN with (tm:=t).
+                destruct (term_trans t) as []eqn:?;automate.
+                rewrite <- Heql. unfold func_term_trans.
+                rewrite <- PeanoNat.Nat.add_succ_comm.
+                rewrite <- app_assoc...
+              * rewrite app_length... rewrite PeanoNat.Nat.add_comm...
+            + repeat (rewrite app_comm_cons).
+              rewrite app_assoc.
+              apply rel_hdl_stk with
+                (frm:=frm) (frm_stk:=frm_stk)...
+              rewrite app_comm_cons. constructor...
+              apply rel_frame with
+                (C_mem:=c_comp S_builtin_ins SC0)
+                (lst:=lst ++ [val_trans r0 v;val_trans r1 v';
+                              call r0])
+                (Ilst:=push r1 :: func_term_trans (S (List.length E1)) t)...
+              * inversion H2...
+              * rewrite H15. cbn. pose proof term_trans_not_nil as NN.
+                specialize NN with (tm:=t).
+                destruct (term_trans t) as []eqn:?;automate.
+                rewrite <- Heql. unfold func_term_trans.
+                rewrite <- PeanoNat.Nat.add_succ_comm.
+                rewrite <- app_assoc...
+              * rewrite app_length... rewrite PeanoNat.Nat.add_comm... }
+        destruct v' as [cst|[ind|str]]...
+        rewrite <- map_nth with (d:=L.ns). rewrite app_nth1...
+        inversion H2... rewrite List.map_length...
+        inversion H6...
+        specialize H4 with (v':=L.var_val ind).
+        assert (Temp:In (L.var_val ind) [L.var_val (L.dbjind_var ind)]).
+        { super_a. } apply H4 in Temp. inversion Temp...
+      * inversion H14... inversion H18.
+        apply H4 in H6. unfold c_comp.
+        rewrite H6. unfold code_mem_trans.
+        rewrite H18...
+      * inversion H14... unfold code_mem_trans in Heqi.
+        rewrite H18 in Heqi...
 (*other things
 0. changes in lexi heaps e.g. assignment
 1. handler related stuff
@@ -888,7 +1316,11 @@ newref's translation s hould be malloc r2 n rather than i
 simplifications can be done:
 sfree after function call is just size of environment,
       no need to compute numlet
-*)
+ *)
+(* new changes after paper submitted
+0. change definition of relating frames
+1. passes parameter C_mem all the way down to frame relation
+2. added well-formed ness for rel_ins rather than at LS_rel *)
 
 
 
